theories/vir/mcfg_contextual.v
@@ -1,0 +1,37 @@
+From iris.prelude Require Import options.
+
+From velliris.program_logic Require Import program_logic.
+From velliris.vir Require Import
+  vir val_rel heapbij adequacy spec globalbij logical_relations fundamental.
+
+From Vellvm Require Import Syntax.DynamicTypes Handlers Syntax.LLVMAst
+  Semantics.InterpretationStack.
+
+From ITree Require Import Recursion.
+
+Import LLVMEvents.
+
+Set Default Proof Using "Type*".
+
+Section mcfg_contextual.
+
+  Context `(sheapGS Σ, checkedoutGS Σ, heapbijGS Σ).
+
+  (* The contextual refinement on [denote_mcfg]. *)
+  Lemma contextual_denote_mcfg :
+    ∀ γ_t γ_s dv dv' e_t e_s main C,
+    □ fun_logrel e_t e_s ∅ -∗
+      checkout ∅ -∗
+      stack_tgt [γ_t] -∗
+      stack_src [γ_s] -∗
+      denote_mcfg ((dv, e_t) :: C) DTYPE_Void (DVALUE_Addr main) []
+      ⪯
+      denote_mcfg ((dv', e_s) :: C) DTYPE_Void (DVALUE_Addr main) []
+      [[ (λ x y : uvalue, ⌜obs_val x y⌝) ⤉ ]].
+  Proof.
+    iIntros (????????) "#Hfun Hc Hs_t Hs_s".
+    rewrite /denote_mcfg.
+
+  Admitted.
+
+End mcfg_contextual.
